\section{Target Estimation} \label{sec:target_estimation}

\begin{align}
  P_{SS,k}(l) &= P_{YY,k}(l) - P_{NN,k}(l)
  \label{eq:psds1} \\
  \widehat{\abs{S_{k}(l)}}^{2} &= \abs{Y_{k}(l)}^{2}-\abs{N_{k}(l)}^{2}
  \label{eq:psds2} \\
  \widehat{\abs{S_{k}(l)}}^{2} &=
  \left(\max{\left\{1-\frac{E\left[\abs{N_{k}(l)}^{2}\right]}{\abs{y_{k}(l)}^{2}},\epsilon\right\}}\right)^{\frac{1}{2}}\abs{y_{k}(l)}
  \label{eq:psds3} \\
  S_{k}(l)^{2} &= \widehat{\abs{S_{k}(l)}}^{2} \dot e^{j\measuredangle y_{k}(l)}
\end{align}

\begin{align}
  \hat{S_{k}} &= H_{k} \dot Y_{k}
  \label{eq:wiener1} \\
  H_{k} &= \frac{P_{SY,k}}{P_{PYY,k}}
  \label{eq:wiener2} \\
  &= \frac{SNR_{k}}{SNR_{k}+1}
  \label{eq:wiener3}
\end{align}
